---
layout: homework
title: "Homework 3"
due-date: 2019-02-15
class: s2019-317
class-name: "Math 317"
assignment: 3
points: 25
solutions: true
---

1. (10.5) Complete the proof of Theorem 10.4 by showing that if $$(s_n)$$ is an
   unbounded decreasing sequence, that $$\lim s_n = -\infty$$.
   
   {:.solution .collapse}
   
   > **Proof.** Let $$(s_n)$$ be an unbounded increasing sequence. Let $$M <
   > 0$$. Since the set $$\{s_n : n \in \mathbb N\}$$ is unbounded and it is
   > bounded above by $$s_1$$, it must be unbounded below. Hence for some $$N
   > \in \mathbb N$$ we have $$s_N < M$$. Also $$n > N$$ implies $$s_n \le s_N <
   > M$$, so $$\lim s_n = -\infty.$$ $$\Box$$
     
2. Let $$(s_n)$$ be a sequence defined by $$s_1 = \sqrt 2$$ and $$s_{n+1} =
   \sqrt{2 + \sqrt {s_n}}$$. Show that $$(s_n)$$ converges to a real number.
   You may use that if $$0 \le a \le b$$ then $$0 \le \sqrt a
   \le \sqrt b$$. (**Hint**: Use the Monotone Convergence Theorem.)
   
   {:.solution .collapse}
   
   > **Proof.** We first prove by induction that $$0 < s_n \le s_{n+1} \le 2$$ for all $$n \in \mathbb N$$. The base case
   > is from that, $$0 < s_1 = \sqrt 2 \le \sqrt{ 2 + \sqrt{\sqrt 2} } = s_2 <
   > \sqrt{4} = 2$$. Suppose now that $$0 < s_k \le s_{k+1} \le 2$$. Then,
   >
   > $$
   > \begin{align*}
   > 0 < s_k &\le s_{k+1} \le 2 \\
   > \sqrt 0 < \sqrt {s_k} &\le \sqrt{s_{k+1}} \le \sqrt 2 \\
   > 2 + \sqrt 0 < 2 + \sqrt {s_k} &\le 2 + \sqrt{s_{k+1}} \le 2 + \sqrt 2 \\
   > \sqrt{2 + \sqrt 0} < \sqrt{2 + \sqrt {s_k}} &\le \sqrt{2 + \sqrt{s_{k+1}}} \le \sqrt{2 + \sqrt 2} \\
   > \sqrt{2} < s_{k+1} &\le s_{k+2} < \sqrt{2+\sqrt 2}
   > \end{align*}
   > $$
   >
   > Notice that this implies then that $$0 < s_{k+1} \le s_{k+2} < 2$$. Hence
   > $$0 < s_n \le s_{n+1} \le 2$$ for all $$n \in \mathbb N$$. This means that
   > $$(s_n)$$ is monotone increasing and bounded, so the Monotone Convergence
   > Theorem for sequences says that it must converge to some real number. $$\Box$$.

3.  (10.8) Let $$(s_n)$$ be an increasing sequence of positive numbers. Let
    $$(\sigma_n)$$ be defined by,
   
    $$
    \sigma_n = \frac{s_1 + s_2 + \cdots + s_n}{n}.
    $$

    Prove that $$(\sigma_n)$$ is in increasing sequence. (The $$\sigma_n$$ are called
    *Cesaro means*)
    
    {:.solution .collapse}
    
    > **Proof.** We will show that $$\sigma_n \le \sigma_{n+1}$$ by showing that
    > $$\sigma_{n+1} - \sigma_n$$ is nonnegative.
    >
    > $$
    > \begin{align*}
    > \sigma_{n+1} - \sigma_n &= \frac{s_1 + s_2 + \cdots + s_n + s_{n+1}}{n+1} +
    > \frac{s_1 + s_2 + \cdots + s_n}{n} \\
    > &= \frac {n(s_1 + s_2 + \cdots + s_n + s_{n+1}) - (n+1)(s_1 + s_2 + \cdots + s_n)}{n(n+1)}
    > \end{align*}
    > $$
    > 
    > As $$n(n+1)$$ is positive, this fraction is nonnegative if its numerator is. So, we examine:
    >
    > $$
    > \begin{align*}
    > n(s_1 + s_2 + \cdots + s_n + s_{n+1}) - (n+1)(s_1 + s_2 + \cdots + s_n) \\
    > &= n(s_1 + s_2 + \cdots + s_n) + ns_{n+1} - n(s_1 + s_2 + \cdots + s_n) - (s_1 + s_2 + \cdots + s_n) \\
    > &= ns_{n+1} - (s_1 + s_2 + \cdots + s_n) \\
    > &= (s_{n+1}-s_1) + (s_{n+1}-s_2) + \cdots + (s_{n+1}-s_n)
    > \end{align*}
    > $$
    > As each of the $$s_{n+1}-s_i$$ is nonnegative as $$s_{n+1} > s_i > 0$$ for each $$1 \le i \le n$$
    > (as $$s_n$$ is positive and increasing) the whole sum is nonnegative. So the numerator is nonnegative, and we conclude that $$\sigma_{n+1} - \sigma_n$$ is nonnegative, so $$\sigma_{n} \le \sigma_{n+1}$$, so $$(\sigma_n)$$ is an increasing sequence. $$\Box$$
    >
 
4.  For each of the following sequences, find the $$\liminf$$ and the
    $$\limsup$$.
   
    1. $$a_n = \frac{(-1)^n}{n}$$
    
        {:.solution .collapse}
    
        > $$\lim a_n = 0$$ so $$\liminf a_n = \limsup a_n = 0$$.
   
    2. $$b_n = n \cos \left( \frac {n\pi}{4} \right)$$
    
        {:.solution .collapse}
    
        > $$\liminf b_n = -\infty$$ and $$\limsup b_n = +\infty$$.
   
    3. $$c_n = (-1)^n + \frac 1n$$
    
        {:.solution .collapse}
    
        > $$\liminf c_n = -1$$ and $$\limsup c_n = 1$$.
 
5. (11.8) Prove that $$\liminf s_n = -\limsup(-s_n)$$ for any sequence $$s_n$$. You
   may use the result of exercise 5.4 without proving it.
   
   {:.solution .collapse}
   
   > **Proof.** We have that :
   >
   > $$
   > \begin{align*}
   > \liminf s_n &= \lim_{N \to \infty} \inf \{ s_n : n > N \} \text{ by definition} \\
   > &= \lim_{N \to \infty} \left( - \sup \{ -s_n : n > N\} \right) \text{ by ex 5.4}\\
   > &= -\lim_{N \to \infty} \left( \sup \{ -s_n : n > N\} \right) \text{ by thm 9.2 and ex 9.10b}\\
   > &= -\limsup{ -s_n }.
   > \end{align*}
   > $$
   >
   > It remains to show the result of exercise 9.10(b) which says that $$\lim
   > s_n = +\infty$$ if and only if $$\lim -s_n = -\infty$$. Suppose that $$\lim
   > s_n = + \infty$$. Suppose that $$M < 0$$. Then there exists $$N$$ so that
   > for all $$n > N$$, $$s_n > -M$$. But this means $$-s_n < M$$. So $$\lim s_n
   > = -\infty$$ for all $$n > N$$ as $$M$$ was arbitrary. The reverse direction
   > follows by a similar argument. $$\Box$$
