---
layout: homework
title: "Homework 4"
due-date: 2019-03-01
class: s2019-317
class-name: "Math 317"
assignment: 4
points: 25
solutions: true
---

1.   (12.4) Show $$\limsup(s_n+t_n) \le \limsup s_n + \limsup t_n$$ for bounded
     sequences $$(s_n)$$ and $$(t_n)$$. You may use the results of Exercise 9.9
     from the book without first proving them. *Hint:* First show
     
     $$
     \sup\{s_n+t_n : n > N\} \le \sup\{s_n:n>N\} + \sup\{t_n:n>N\}
     $$
     
     and then apply Exercise 9.9(c).
     
     {::options parse_block_html="true" /}
     
     <div class="solution collapse">
     
     **Proof.** Let $$N > 0$$ and consider $$k > N$$. As
     $$s_k \in \{s_n:n>N\}$$, $$s_k \le \sup\{s_n:n>N\}$$. Similarly,
     $$t_k \le \sup\{t_n:n>N\}$$. So,
     
     $$
     s_k + t_k \le \sup\{s_n:n>N\} + \sup\{t_n:n>N\},
     $$
     
     so that $$\sup\{s_n:n>N\} + \sup\{t_n:n>N\}$$ is an upper bound for the set
     $$\{s_n + t_n:n>N\}$$. In particular, this means that
     
     $$
     \sup\{s_n + t_n:n>N\} \le \sup\{s_n:n>N\} + \sup\{t_n:n>N\}.
     $$
     
     Taking limits as $$N \to \infty$$ of both sides preserves the inequality
     (this is the result of Exercise 9.9(c)), so that
     
     $$
     \begin{align*}
     \lim_{N\to\infty}\sup\{s_n + t_n:n>N\} &\le \lim_{N\to\infty}(\sup\{s_n:n>N\} + \sup\{t_n:n>N\}) \\
     &= \lim_{N\to\infty}\sup\{s_n:n>N\} + \lim_{N\to\infty}\sup\{t_n:n>N\},
     \end{align*}
     $$
     
     and applying the definition of $$\limsup$$ yields,
     
     $$
     \limsup s_n \le \limsup s_n + \limsup t_n,
     $$

     as claimed. $$\Box$$
     
     </div>

2.   (12.12) **This question is worth double points**. Let $$(s_n)$$ be any sequence
     of non-negative real numbers. Let $$(\sigma_n)$$ be defined by,
   
     $$
     \sigma_n = \frac{s_1 + s_2 + \cdots + s_n}{n}.
     $$

     1.  Show
     
         $$
         \liminf s_n \le \liminf \sigma_n \le \limsup \sigma_n \le \limsup s_n
         $$
         
         *Hint:* For the last inequality, show first that $$M > N$$ implies
         
         $$
         \sup \left\{\sigma_n : n > M\right\} \le 
         \frac 1M \left(s_1+s_2+\cdots+s_N\right) +
         \sup \left\{ s_n : n > N \right\}
         $$
         
         {::options parse_block_html="true" /}
     
         <div class="solution collapse">
         
         **Proof.** We have trivially that $$\liminf \sigma_n \le \limsup
         \sigma_n$$, so we need only prove the first and last inequalities.
         First we will prove the inequality:
         
         $$\limsup \sigma_n \le \limsup s_n.$$
         
         Consider $$N > 0$$ and any $$M > N$$. Consider any $$k > M$$. We will
         bound $$\sigma_k$$ from above:
         
         $$
         \begin{align}
         \sigma_k &= \frac 1k \sum_{i=1}^{k}{s_i} \\
         &= \frac 1k \sum_{i=1}^{N}{s_i} + \frac 1k \sum_{i={N+1}}^{k}{s_i} \\
         &\le \frac 1M \sum_{i=1}^{N}{s_i} + \frac 1k \sum_{i={N+1}}^{k}{\sup\{s_n : n > N\}},
         \end{align}
         $$
         
         where we have used that (1) $$\sum_{i=1}^{N}{s_i} \ge 0$$ as all $$s_n$$ are nonnegative, (2) $$1/k < 1/M$$, and (3) that
         for all $$N+1 < i < k$$ we have $$s_i \le \sup\{s_n : N > N\}$$. So,
         
         $$
         \begin{align}
         \sigma_k &\le \frac 1M \sum_{i=1}^{N}{s_i} + \frac {k-N}{k} {\sup\{s_n : n > N\}} \\
         &\le \frac 1M \sum_{i=1}^{N}{s_i} + {\sup\{s_n : n > N\}},
         \end{align}
         $$
         
         As $$\frac{k-N}k \le 1$$. This upper bound holds for all $$k > M$$, so we may conclude that
         
         $$
         \sup\{\sigma_n : n > M\} \le \frac 1M \sum_{i=1}^{N}{s_i} + {\sup\{s_n : n > N\}}.
         $$
         
         As this relationship holds for all $$M > N$$, taking limits of either
         side as $$M \to \infty$$ (we may do this as increasing $$M$$ preserves
         the property that $$M > N$$) we obtain,
         
         $$
         \begin{align}
         \lim_{M\to\infty}\sup\{\sigma_n : n > M\} &\le 
         \lim_{M\to\infty}\left(\frac 1M \sum_{i=1}^{N}{s_i}\right) + \lim_{M\to\infty}{\sup\{s_n : n > N\}} \\
         &\le 0 + \sup\{s_n : n > N\}, \\
         \end{align}
         $$
         
         so that $$\limsup{\sigma_n} \le \sup\{s_n : n > N\}$$.
         
         Taking limits then as $$N \to \infty$$ we get that
         
         $$
         \begin{align}
         \lim_{N \to \infty}\limsup \sigma_n &\le \lim_{N \to \infty}\sup\{s_n : n > N\} \\
         \limsup \sigma_n &\le \limsup {s_n}
         \end{align}
         $$
         
         as desired.
         
         We now show the first inequality, which uses similar techniques but is
         slightly different. We take $$N > 0$$, any $$M > N$$, and consider 
         arbitrary $$k > M$$. Then we examine a lower bound for $$\sigma_k$$;
         
         $$
         \begin{align}
         \sigma_k &= \frac 1k \sum_{i=1}^{k}{s_i} \\
         &= \frac 1k \sum_{i=1}^{N}{s_i} + \frac 1k \sum_{i={N+1}}^{k}{s_i} \\
         &\ge 0 + \frac 1k \sum_{i={N+1}}^{k}{\inf\{s_n : n > N\}} \\
         &= \frac{k-N}{k}\inf\{s_n : n > N\},
         \end{align}
         $$
         
         where we have used that (1) $$\sum_{i=1}^{N}{s_i} \ge 0$$ as all
         $$s_n$$ are nonnegative, and (2) that for all $$N+1 < i < k$$ we have
         $$s_i \ge \inf\{s_n : N > N\}$$. Notice now that $$\frac{k-N}{k} = 1 -
         \frac Nk \ge 1 - \frac NM$$, so that
         
         $$
         \sigma_k \ge \left(1 - \frac NM\right)\inf\{s_n : n > N\}.
         $$
         
         This lower bound holds for all $$k > M$$ so we have proved that
         
         $$
         \inf\{\sigma_n : n > M\} \ge \left(1 - \frac NM\right)\inf\{s_n : n > N\}.
         $$
         
         Similar to before, taking limits as $$M \to \infty$$ yields that
         
         $$
         \liminf \sigma_n \ge \inf\{s_n : n > N\},
         $$
         
         and taking limits as $$N \to \infty$$ yields finally that
         
         $$
         \liminf \sigma_n \ge \liminf s_n,
         $$
         
         as desired. $$\Box$$
         
         </div>
         
     2.  Show that if $$\lim_{n\to\infty} s_n$$ exists, then $$(\sigma_n)$$
         converges and $$\lim_{n\to\infty} \sigma_n = \lim_{n\to\infty} s_n$$
         
         {::options parse_block_html="true" /}
     
         <div class="solution collapse">
         
         **Proof.** If $$\lim s_n$$ exists then $$\lim s_n = \liminf s_n = \limsup s_n$$ and so by (a)
         $$\lim s_n = \liminf \sigma_n = \limsup \sigma_n = \lim \sigma_n$$. $$\Box$$
         
         </div>
         
     3.  Give an example of a sequence $$(s_n)$$ so that $$(\sigma_n)$$
         converges but $$(s_n)$$ does not.
         
         {::options parse_block_html="true" /}
     
         <div class="solution collapse">
         
         Here is one example:
         
         Let $$s_n = (-1)^n$$. Then $$(s_n)$$ diverges, but what of
         $$\sigma_n$$? For even $$n$$ we can see that $$\sigma_n = 0$$ and odd
         $$n$$ we have that $$\sigma_n = -\frac 1n$$. This means that $$\limsup
         \sigma_n = \lim 0 = 0$$ and $$\liminf \sigma_n = \lim \left(-\frac
         1n\right) = 0$$ and we conclude that $$\lim \sigma_n = 0$$.
         
         </div>
         
3.   (14.1--4) For each of the following, determine whether the given series
     converges and justify your answer.
     
     1.  $$\sum{\frac {n^3}{3^n}}$$
     
         {::options parse_block_html="true" /}
     
         <div class="solution collapse">
         
         Converges by the ratio test. We have the ratios
         $$\frac{(n+1)^3}{3^{n+1}}\frac{3^n}{n^3} = \frac{(n+1)^3}{3n^3}$$,
         whose $$n \to \infty$$ limit is $$1/3 < 1$$.
         
         </div>
     
     2.  $$\sum{\frac {1}{2^n + n}}$$
     
         {::options parse_block_html="true" /}
     
         <div class="solution collapse">
         
         Converges by comparison, as $$\frac{1}{2^n + n} < \frac{1}{2^n}$$ whose
         corresponding series is a convergent geometric series.
         
         </div>
     
     3.  $$\sum{ \frac{n!}{n^n} }$$
     
         {::options parse_block_html="true" /}
     
         <div class="solution collapse">
         
         Converges by the ratio test. We have the ratios
         
         $$
         \frac{(n+1)!}{(n+1)^{n+1}}\frac{n^n}{n!} = \frac{(n+1)n^n}{(n+1)^{n+1}} = \left(\frac{n}{n+1}\right)^n
         $$
         
         whose $$n \to \infty$$ limit is $$1/e < 1$$.
         
         </div>

4.   (14.8) Show that if $$\sum a_n$$ and $$\sum b_n$$ are convergent series of
     nonnegative numbers, then $$\sum \sqrt{a_n b_n}$$ converges. *Hint:* Show
     $$\sqrt{a_n b_n} \le a_n + b_n$$ for all $$n$$.
     
     {::options parse_block_html="true" /}
     
     <div class="solution collapse">
     
     **Proof.** We claim that $$\sqrt{a_n b_n} < a_n + b_n$$, from which
     convergence of the series follows from the comparison test.
     
     Observe that as both $$a_n$$ and $$b_n$$ are nonnegative,
     
     $$
     \begin{align}
     a_n^2 + a_nb_n + b_n^2 &\ge 0 \\
     a_n^2 + 2a_nb_n + b_n^2 &\ge a_nb_n \\
     (a_n + b_n)^2 &\ge a_nb_n \\
     a_n + b_n &\ge \sqrt{a_nb_n},
     \end{align}
     $$
     
     proving the claim. $$\Box$$
     
     <div>
