---
layout: homework
title: "Homework 8"
due-date: 2019-04-12
class: s2019-317
class-name: "Math 317"
assignment: 8
points: 20
solutions: true
---

1.  (29.4) Let $$f$$ and $$g$$ be differentiable functions on an open interval
    $$I$$. Suppose there are $$a,b \in I$$ with $$a < b$$ and $$f(a) = f(b) =
    0$$. Show that there exists $$x \in I$$ so that
    
    $$
    f'(x) + f(x)g'(x) = 0.
    $$
    
    *Hint*. Consider $$h(x) = f(x) e^{g(x)}$$.
    
    {::options parse_block_html="true" /}
    
    <div class="solution collapse">
    
    **Proof**. Let $$h(x) = f(x) e^{g(x)}$$, so that $$h'(x) = f'(x) e^{g(x)} +
    f(x) e^{g(x)} g'(x) = e^{g(x)}(f'(x) - f(x) g'(x))$$. By Rolle's theorem, as
    $$h(a) = h(b) = 0$$, there exists $$c$$ between $$a, b$$ so that $$h(c) =
    0$$. But as $$e^{g(x)} \ne 0$$ always, this implies that $$f'(c) - f(c) g'(c) = 0$$.

    </div>
    
2.  (31.2) Consider the *hyperbolic sine and cosine* functions, $$\sinh(x) =
    \frac{e^x - e^{-x}}{2}$$ and $$\cosh(x) = \frac{e^x + e^{-x}}{2}$$.
    
    1.  Find the Taylor series for $$\sinh(x)$$ and show that it converges to $$\sinh(x)$$.
    
    2.  Find the Taylor series for $$\cosh(x)$$ and show that it converges to $$\cosh(x)$$.
    
    {::options parse_block_html="true" /}
    
    <div class="solution collapse">
    
    1.  We have that $$\sinh'(x) = \frac{e^x + e^{-x}}2 = \cosh(x)$$ and that
        $$\cosh'(x) = \sinh(x)$$ by basic calculation. Let $$c = 0$$ be where we
        center our Taylor series, and notice that $$\sinh(0) = 0$$ and
        $$\cosh(0) = 1$$. So using the formula for Taylor series, we get that
        the Taylor series for $$\sinh(x)$$ is,
        
        $$
        \sum_{n=1}^\infty {\frac{x^{2n+1}}{(2n+1)!}}
        $$
        
        Let $$M > 0$$ and consider the interval $$(-M, M)$$. Notice that
        $$\sinh(x) = \frac 12 (\vert e^x - e^{-x} \vert) \le \frac 12 (e^x +
        e^x) \le e^M$$ on the interval $$(-M, M)$$. By a similar argument,
        $$\cosh(x) \le e^M$$ on $$(-M, M)$$. By the Corollary to Taylor's
        theorem, we deduce that $$\sinh$$ converges to its Taylor series on
        $$(-M, M)$$. $$M> 0$$ is arbitrary, so we may in fact deduce that
        $$\sinh$$ converges to its Taylor series on all of $$\mathbb R$$.
        
    2.  The Taylor series for $$\cosh(x)$$ is,
    
        $$
        \sum_{n=1}^\infty {\frac{x^{2n}}{(2n)!}}
        $$
        
        and the argument for showing that it converges to $$\cosh$$ on $$\mathbb
        R$$ is identical to part (a).
    
    </div>
    
3.  (31.6) We're going to work through an alternative proof of Taylor's theorem,
    for Taylor series centered at $$c = 0$$.
    
    Let $$f$$ be defined on $$(a, b)$$ with $$a < 0 < b$$ and assume that, for
    given $$n \in \mathbb N$$, $$f^{(n)}$$ exists on $$(a, b)$$. Let $$x > 0$$,
    and take $$M$$ to be the unique number so that
    
    $$
    f(x) = \sum_{k=0}^{n-1}{\frac{f^{(k)}(0)}{k!} x^k + \frac{Mx^n}{n!}}
    $$

    is valid. Define
    
    $$
    F(t) = f(t) + \sum_{k=1}^{n-1}{\frac{(x-t)^k}{k!}f^{(k)}(t) + M\frac{(x-t)^n}{n!}}
    $$
    
    for $$t \in [0, x]$$. **An earlier version had a typo, saying that $$F$$ was
    a function of $$x$$, instead of $$t$$. The version now is correct.**
    
    1.  Show that $$F$$ is differentiable on $$[0, x]$$ and that furthermore
    
        $$
        F'(t) = \frac{(x-t)^{n-1}}{(n-1)!}[f^{(n)}(t) - M].
        $$
        
    2.  Show $$F(0) = F(x)$$.
    
    3.  Apply Rolle's Theorem to obtain $$y \in (0, x)$$ so that $$f^{(n)}(y) = M$$.
    
    {::options parse_block_html="true" /}
    
    <div class="solution collapse">
    
    1.  This is a simple calculation. With care, you will notice that all
        interior terms in the sum cancel to yield the desired expression.
        
    2.  A calculation shows that $$F(0) = f(x) = F(x)$$.
    
    3.  As $$F(0) = F(x)$$ there exists $$0 < y < x$$ for which $$F'(y) = 0$$ by
        Rolle's theorem. $$F'(y) = 0$$ implies that $$f^{(n)}(y) - M = 0$$, from
        which we conclude that $$f^{(n)}(y) = M$$.
    
    </div>

4.  Let $$f$$ be differentiable on $$\mathbb R$$ with $$a = \sup\{ \vert f'(x) \vert : x \in \mathbb R \} < 1$$.

    1.  Select $$s_0 \in \mathbb R$$ and define $$s_n = f(s_{n-1})$$ for $$n \ge 1$$.
    
        Prove that $$(s_n)$$ is a convergent sequence. *Hint*. To show that
        $$(s_n)$$ is Cauchy, first show that $$\vert s_{n+1} - s_n \vert \le a
        \vert s_n - s_{n-1}\vert$$ for $$n \ge 1$$.
        
    2.  Show that $$f$$ has a *fixed point*. In other words, there is a number
        $$s$$ so that $$f(s) = s$$.
        
    {::options parse_block_html="true" /}
    
    <div class="solution collapse">
    
    1.  **Proof**. Consider the interval from $$s_{n-1}$$ to $$s_n$$. The Mean Value
        Theorem says that there exists a number $$c$$ between $$s_{n-1}$$ and
        $$s_n$$ so that
        
        $$
        \left\vert\frac{s_{n+1} - s_n}{s_n - s_{n-1}}\right\vert
        = \left\vert\frac{f(s_n) - f(s_{n-1})}{s_n - s_{n-1}}\right\vert = \vert f'(c)\vert \le a < 1.
        $$
        
        In particular, we have that $$\vert s_{n+1} - s_n \vert \le a\vert s_n -
        s_{n-1}\vert$$. From this, iterated, we see that for all $$N \in \mathbb
        N$$, $$\vert s_{N+1} - s_N \vert \le a^N \vert s_1 - s_0 \vert$$. The series
        $$\sum_{k=1}^\infty a^k$$ is convergent as $$a < 1$$, and say its value is $$A$$.
        
        Let $$\epsilon < 0$$ and consider a natural number $$N > \frac{\log
        (\epsilon/(A\vert s_1 - s_0 \vert))}{\log a}$$. Then for $$n, m > N$$ we
        have that
        
        $$
        \begin{align*}
        \vert s_n - s_m\vert &= \left\vert \sum_{k=m+1}^{n}{s_k - s_{k-1}} \right\vert \\
        &\le \sum_{k=m+1}^n {\vert s_k - s_{k-1} \vert} \\
        &\le \sum_{k=m+1}^n a^k {\vert s_1 - s_{0} \vert} \\
        & = a^N \vert s_1 - s_0 \vert\sum_{k=m+1}^n {a^{k-N}} \\
        &\le a^N \vert s_1 - s_0 \vert A < \epsilon.
        \end{align*}
        $$
        
        So $$(s_n)$$ converges.
    
    2. Let $$\lim s_n = s$$. Then notice that as $$f$$ is differentiable, hence
       continuous, $$\lim_{n\to \infty} f(s_n) = f(\lim_{n\to \infty} s_n) = f(s)$$ but also that
       $$\lim_{n\to \infty} f(s_n) = \lim_{n\to \infty} s_{n+1} = s$$. So $$f(s) = s$$.
    
    </div>
