---
layout: homework
title: "Homework 1"
due-date: 2019-09-06
class: f2019-317
class-name: "Math 317"
class-uids: 
  - 89757
assignment: 1
points: 25
solutions: true
---

You are welcome to use any result of Theorem 3.1 and 3.2 in the book if you find
them helpful.

1.  Prove that $$1^3 + 2^3 + 3^3 + \cdots + n^3 = (1 + 2 + 3 + \cdots + n)^2$$.

    {::options parse_block_html="true" /}
    
    <div class="solution collapse">
    
    We prove this using induction. As a base case, we notice that \\(1^3 = 1 = (1)^2\\).
    
    Suppose now that \\(1^3 + 2^3 + \cdots + k^3 = (1 + 2 + \cdots k)^2\\). Then:
    
    $$
    \begin{align*}
    1^3 + 2^3 + \cdots + k^3 + (k+1)^3
    &= (1^3 + 2^3 + \cdots + k^3) + (k+1)^3 \\
    &= (1 + 2 + \cdots k)^2 + (k+1)^3 \\
    &= \left(\frac{k(k+1)}2\right)^2 + (k+1)^3 \\
    &= (k+1)^2\left(\frac{k^2}4 + (k+1)\right) \\
    &= (k+1)^2\left(\frac{k^2+4k+4}4\right) \\
    &= (k+1)^2\left(\frac{(k+2)^2}4\right) \\
    &= \left(\frac{(k+1)((k+1)+1)}2\right)^2 \\
    &= (1 + 2 + \cdots (k+1))^2
    \end{align*}
    $$
    
    So we are done by induction.
    
    </div>
    
2.  Guess a formula for the sum $$1 + 3 + \cdots + (2n - 1)$$ (try evaluating
    for $$n = 1,2,3,4$$ and look for patterns). Then prove that your formula is
    correct.
    
    {::options parse_block_html="true" /}
    
    <div class="solution collapse">
    
    We claim that \\(1 + 3 + \cdots + (2n - 1) = n^2\\).
    
    We prove this using induction. As a base case, we notice that \\(1 = 1^2\\).
    
    Suppose now that \\(1 + 3 + \cdots + (2k - 1) = k^2\\). Then:
    
    $$
    \begin{align*}
    1 + 3 + \cdots + (2k - 1) + (2k + 1)
    &= (1 + 3 + \cdots + (2k - 1)) + (2k + 1) \\
    &= k^2 + (2k - 1)\\
    &= (k+1)^2
    \end{align*}
    $$
    
    So we are done by induction.
    
    </div>

3.  For each subset of $$\mathbb R$$ below, determine both the
    **maximum** and the **minimum**, if they exist. If either doesn't exist,
    say so. You do not need to give a rigorous proof of your answer.
    
    1.  $$A = \{ 3, 5, 1, 4 \}$$
    
    2.  $$B = \left\{\dfrac {(-1)^n}n \;:\; n \in \mathbb N \right\}$$
    
    3.  $$C = \left\{\cos\left(\dfrac{n\pi}{3}\right) \;:\; n \in \mathbb N \right\}$$
    
    4.  $$D = \{ r \;:\; r \in \mathbb Q,\; r^2 < 5 \}$$
    
    5.  $$E = \left\{ 1 - \dfrac{1}{2^n} \;:\; n \in \mathbb N \right\}$$
    
    {::options parse_block_html="true" /}
    
    <div class="solution collapse">
    
    1.  Maximum 5, minimum 1
    
    2.  Maximum 1/2, minimum -1
    
    3.  Maximum 1, minimum -1
    
    4.  Maximum DNE, minimum DNE
    
    5.  Maximum DNE, minimum 1/2
    
    </div>
    
4.  Don't worry about writing out any formal proofs in this problem. Decide
    whether each of the following statements is true. If the statement is **true**,
    you don't need to do anything more. If the statement is **false**, give a
    concrete example (that is, a counterexample) that shows the statement
    failing.
    
    1.  An **irrational** number is an element of $$\mathbb R \setminus \mathbb Q$$. If $$r \ne 0$$ is rational and $$\alpha$$ is irrational, then
        $$r + \alpha$$ is irrational.
        
    2.  $$\vert \vert a \vert - \vert b \vert \vert \le \vert a - b \vert$$ for all $$a, b \in \mathbb R$$.
        
    3.  A nonempty finite set always has a maximum.
    
    {::options parse_block_html="true" /}
    
    <div class="solution collapse">
    
    1.  True. If \\(r + \alpha = p/q\\) for some integers \\(p, q\\) then \\(\alpha = p/q - r\\), a rational; this is a contradiction.
    
    2.  True. Without loss of generality, assume that \\(\vert a \vert \ge \vert b \vert\\) so that \\(\vert \vert a \vert - \vert b \vert \vert = \vert a \vert - \vert b \vert\\). We have that \\(\vert a \vert = \vert (a-b) + b \vert \le \vert a-b \vert + \vert b \vert\\) by the Triangle inequality, which is equivalent to saying that \\(\vert a \vert - \vert b \vert \le \vert a - b \vert\\).
    
    3.  True. This is a fact about maximums; since the set is finite, a maximum can always be found in finite time (just look through all elements).
    
    </div>
    
    
5.  Let $$A$$ be a nonempty set of real numbers which has a minimum. Let
    $$-A$$ be the set $$\{ -x \;:\; x \in A \}$$. Prove that
    
    $$
    \min A = -\max(-A).
    $$
    
    {::options parse_block_html="true" /}
    
    <div class="solution collapse">
    
    Let \\(m = \min A\\). So for each \\(a \in A, m \le a\\). Then for any \\(y=-a \in -A\\), we have that \\(m \le a\\) and so \\(-m \ge -a = y\\). So \\(-m = \max (-A)\\) or equivalently that \\(\min A = -\max(-A)\\).
    
    </div>
