---
layout: homework
title: "Homework 3"
due-date: 2019-09-20
class: f2019-317
class-name: "Math 317"
class-uids: 
  - 89757
assignment: 3
points: 25
solutions: true
---

**Reading**: 
1.  If you haven't yet, skim sections 1, 2, 3, 4, and 7.

2.  Read sections 5, **8**, and 9. (Section 8 is about writing good proofs!)
^

**Exercises**:

1.  Suppose \\(\lim a_n = a\\) and \\(\lim b_n = b\\). Find 
    \\[ \lim \frac{a_n^3 + 4a_n}{b_n^2 + 1} \\]
    and prove that your limit is correct. For this problem, be explicit about which limit theorems you are using for full credit.
    
    {::options parse_block_html="true" /}
    
    <div class="solution collapse">
    
    By the multiplicative law for limits (and also the constant multiple law for limits), \\(\lim a_n^3 = \lim a_n a_n a_n = a^3\\), \\(\lim 4a_n = 4a\\), and \\(\lim b_n^2 = \lim b_n b_n = b^2\\). Then by the additive law for limits \\(\lim (a_n^3 + 4a_n) = a^3 + 4a\\) and \\(\lim (b_n^2 + 1) = b^2 + 1\\). Finally, by the quotient law for limits, **as \\(b_n^2 + 1 > 0\\) and \\(b^2 + 1 > 0\\)**, the limit of the quotient is precisely
    
    \\[ \frac {a^3 + 4a}{b^2 + 1} \\]
    
    </div>

2.  Suppose \\((s_n)\\) is a sequence and \\(0 < s_n < \sqrt{\frac{2}{n-1}} \\) for all \\(n\\). Prove that
    \\[ \lim s_n = 0. \\]
    
    {::options parse_block_html="true" /}
    
    <div class="solution collapse">
    
    We have that \\(\lim 1/n = 0\\), and hence by limit laws we can deduce that \\(\lim \sqrt{\frac{2}{n-1}} = 0\\). Also, \\(\lim 0 = 0\\). So by the squeeze theorem, \\(\lim s_n = 0\\).
    
    </div>


3.  For each of the following false statements, give a counterexample.

    1.  If the sequence $$s_n$$ converges and the sequence $$t_n$$ diverges, the product $$s_nt_n$$ also diverges.

    2.  If $$s_n$$ and $$t_n$$ are two divergent sequences, their sum $$s_n + t_n$$ also diverges.
   
    3.  If a sequence $$s_n$$ converges, so too does the sequence $$t_n = \sum_{i=1}^n{s_i}$$.
    
    {::options parse_block_html="true" /}
    
    <div class="solution collapse">
    
    1.  Take for instance \\((s_n) = (0)\\) and any sequence \\((t_n)\\).
    
    2.  Take for instance any divergent sequence \\((t_n)\\) and \\((s_n) = (-t_n)\\).
    
    3.  Take for instance \\((s_n) = (1)\\).
    
    </div>

4.  Show that if \\(\lim s_n = +\infty\\) and \\(\lim t_n > -\infty\\), then \\(\lim(s_n + t_n) = +\infty\\).

    {::options parse_block_html="true" /}
    
    <div class="solution collapse">
    
    Since \\((t_n)\\) exists and is greater than \\(-\infty\\), the sequence \\((t_n)\\) is bounded below by some number, say \\(L\\).
    
    Let \\(M \in \mathbb R\\) (we think of \\(M\\) as being arbitrarily large). Then as \\(\lim s_n = +\infty\\), there exists \\(N\\) so that \\(n \ge N\\) implies that \\(s_n > M - L\\). Now notice that we've found \\(N\\) so that \\(n \ge N\\) implies that \\(s_n + t_n \ge s_n + L > M - L + L = M\\). So by definition \\(\lim (s_n + t_n) = +\infty\\).
    
    </div>

    
5.  Use the Monotone Convergence Theorem to show that the sequence \\((s_n)\\)
    defined by \\(s_1 = 1\\) and \\(s_{n+1} = \sqrt{s_n + 2}\\) converges.

    {::options parse_block_html="true" /}
    
    <div class="solution collapse">
    
    The sequence \\((s_n)\\) is bounded from below by 0 and above, say, by 10 as \\(s_1 = 1 < 10\\) and if we assume that \\(s_n \le 10\\), we find that \\(s_{n+1} = \sqrt{s_n + 2} \le \sqrt{12} < 10\\).
    
    The sequence \\((s_n)\\) is increasing as \\(s_1 = 1 \le s_2 = \sqrt{1+2}\\) and, if we assume that \\(s_{n-1} \le s_n \\) we see that \\(\sqrt{s_{n-1}+2} \le \sqrt{s_n + 2}\\) and equivalently that \\(s_n \le s_{n+1}\\).
    
    So by the Monotone Convergence Theorem, \\((s_n)\\) must converge.
    
    </div>
